Cleanup and comments of everything except for constructions.

src/Language/STLC/Dynamics/IdSubst.v
@@ -9,16 +9,15 @@ From PlutusCert Require Import
   variables
   psubs.
 
-
+(* Identity subsitutions, where the term is always a variable equal to the key *)
 Inductive IdSubst : list (string * term) -> Set :=
   | id_subst_nil : IdSubst nil
-  | id_subst_cons : forall x sigma , IdSubst sigma -> IdSubst ((x, tmvar x)::sigma).
+  | id_subst_cons : forall x σ , IdSubst σ -> IdSubst ((x, tmvar x)::σ).
 
-
+(* Identity substitutions have no effect *)
 Lemma id_subst__id s σ :
-  (* NC s σ ->  *)
   IdSubst σ -> 
-  psubs σ s = s. (* even when this capturs, it doesnt matter, since it captures something and then substiutes it for the same name*)
+  psubs σ s = s. (* No need for a no-capture premise: even when this "captures", it doesnt matter, since it captures something and then substiutes it for the same name*)
 Proof.
   intros.
   induction s.
@@ -38,47 +37,50 @@ Proof.
 Qed.
 
 
-(* Identity substitutions: Given a typing context E, give a list of term substitutions matching this E*)
-Fixpoint id_subst (E : list (string * PlutusIR.kind)) : list (string * term) :=
-  match E with
+(* Procedure for generating an identity substitution for each name in the kinding context *)
+Fixpoint id_subst (Δ : list (string * PlutusIR.kind)) : list (string * term) :=
+  match Δ with
   | nil => nil
-  | cons (x, A) E' => cons (x, tmvar x) (id_subst E')
+  | cons (x, A) Δ' => cons (x, tmvar x) (id_subst Δ')
   end.
 
-
-Lemma id_subst_is_IdSubst E :
-  IdSubst (id_subst E).
+(* Procedure id_subst really produces identity substitutions*)
+Lemma id_subst_is_IdSubst Δ :
+  IdSubst (id_subst Δ).
 Proof.
-  induction E.
+  induction Δ.
   - constructor.
   - simpl. destruct a. constructor. assumption.
 Qed.
 
-Lemma remove_ids_IdSubst_is_nil sigma :
-  IdSubst sigma -> remove_ids sigma = nil.
+(* An IdSubst only contains identity substitutions *)
+Lemma remove_ids_IdSubst_is_nil σ :
+  IdSubst σ -> remove_ids σ = nil.
 Proof.
   intros.
-  induction sigma.
+  induction σ.
   - reflexivity.
   - simpl.
     destruct a as [x1 x2].
     inversion H; subst.
-    rewrite IHsigma; auto.
+    rewrite IHσ; auto.
     rewrite String.eqb_refl. auto.
 Qed.
 
-Lemma IdSubst_no_binders sigma :
-  IdSubst sigma -> btv_env sigma = nil.
+(* An IdSubst has no binders (no abstraction terms)*)
+Lemma IdSubst_no_binders σ :
+  IdSubst σ -> btv_env σ = nil.
 Proof.
   intros.
-  induction sigma.
+  induction σ.
   - reflexivity.
   - simpl.
     destruct a as [x1 x2].
     inversion H; subst.
-    rewrite IHsigma; auto.
+    rewrite IHσ; auto.
 Qed.
 
+(* An IdSubst behaves the same when applied sequentially or parallelly*)
 Lemma id_subst__ParSeq :
   forall (σ : list (string * term)), IdSubst σ -> ParSeq σ.
 Proof.
@@ -93,24 +95,26 @@ Proof.
       rewrite IdSubst_no_binders; eauto.
 Qed.
 
-Lemma no_btv_in_id_subst E :
-  forall x, In x (btv_env (id_subst E)) -> False.
+(* Helper: For any kinding context, if we generate an identity substitution from it, it does not contain any binders *)
+Lemma no_btv_in_id_subst Δ :
+  forall x, In x (btv_env (id_subst Δ)) -> False.
 Proof.
   intros.
-  induction E.
+  induction Δ.
   - simpl in H. contradiction.
   - simpl in H. destruct a as [x1 x2].
     simpl in H.
-    eapply IHE. auto.
+    eapply IHΔ. auto.
 Qed.
 
-Lemma id_subst__nc_BU E s :
-  NC s (id_subst E) -> BU (id_subst E) s.
+(* If an identity substitution does not cause capture, then BU: the binders in the subsitution are trivially unique and not equal to any in s*)
+Lemma id_subst__nc_BU Δ s :
+  NC s (id_subst Δ) -> BU (id_subst Δ) s.
 Proof.
   intros.
   unfold BU.
   split.
-  - intros. apply no_btv_in_id_subst in H0. contradiction.
+  - intros.  apply no_btv_in_id_subst in H0. contradiction.
   - intros. apply no_btv_in_id_subst in H0. contradiction.
 Qed.
 
