src/Language/STLC/Dynamics/step_naive.v
@@ -6,18 +6,19 @@ From PlutusCert Require Import STLC util variables Util
 
 Local Open Scope string_scope.
 
+(* Naive substitutions that do not prevent capture *)
 Fixpoint sub (X : string) (U T : term) : term :=
   match T with
   | tmvar Y =>
     if X =? Y then U else tmvar Y
   | @tmabs B Y K1 T' =>
-    @tmabs B Y K1 (sub X U T') (* X can never be equal to Y due to GU: We only ever do substitutions such that NC T [(X, U)]*)
+    @tmabs B Y K1 (sub X U T') (* No check if X = Y, because not possible for naive substitutions that cannot cause capture. *)
   | @tmbin B T1 T2 =>
     @tmbin B (sub X U T1) (sub X U T2)
   | tmbuiltin d => tmbuiltin d
   end.
 
-
+(* A single substitution is also a parallel substitution *)
 Lemma single_subs_is_psub X T s :
   psubs [(X, T)] s = sub X T s.
 Proof.
@@ -29,6 +30,7 @@ Proof.
   - simpl. reflexivity.
 Qed.
 
+(* Substituting a name x for a type t, makes x no longer free*)
 Lemma sub_helper {x t s} :
   ~ In x (ftv t) -> ~ In x (ftv (sub x t s)).
 Proof.
@@ -50,7 +52,8 @@ Proof.
   - simpl. auto.
 Qed.
 
-(* need also handle btv, since substitution is nto capture avoiding*)
+(* If x does not occur, the subsitution does not do anything *)
+(* NOTE: need also handle btv, since substitution is not capture avoiding*)
 Lemma sub_vac x t s :
  ~ In x (ftv s) ->
  ~ In x (btv s) ->
@@ -73,8 +76,8 @@ Proof.
     + eapply IHs2; eauto.
       eapply not_ftv_app_not_right; eauto. eapply not_btv_dc_appr. eauto.
 Qed.
-(* looks like sub_vacuous maybe?*)
 
+(* Naive reduction without capture-avoiding beta reduction *)
 Inductive step_naive : term -> term -> Set :=
 | step_beta (x : string) (A : PlutusIR.kind) (s t : term) :
     step_naive (@tmbin App (@tmabs Lam x A s) t) ( sub x t s)
@@ -85,7 +88,7 @@ Inductive step_naive : term -> term -> Set :=
 | step_abs B x A s1 s2 :
     step_naive s1 s2 -> step_naive (@tmabs B x A s1) (@tmabs B x A s2).
 
-
+(* Naive reduction does not introduce free variables *)
 Lemma step_naive_preserves_no_ftv x t1 t2 :
   step_naive t1 t2 -> ~ In x (ftv t1) -> ~ In x (ftv t2).
 Proof.
