src/PlutusIR/Semantics/Static/Normalization/Normalizer.v
@@ -1,15 +1,15 @@
 From PlutusCert Require Import 
   PlutusIR 
-  Normalisation.BigStep
+  Normalization.BigStep
   Kinding.Kinding
   Kinding.Checker
-  Normalisation.SmallStep
+  Normalization.SmallStep
   Util
   SubstituteTCA
   SN_PIR
   SN_STLC_GU
   Progress
-  Normalisation.Preservation.
+  Normalization.Preservation.
 
 Require Import mathcomp.ssreflect.ssreflect.
 Require Import Coq.Lists.List.
@@ -48,33 +48,36 @@ Proof.
 Defined.
 
 (* A gas powered normalizer that does not use the strong normalization result*)
-Fixpoint normaliser_gas (n : nat) {T Δ K} (Hwk : Δ |-* T : K) :=
+Fixpoint normalizer_gas (n : nat) {T Δ K} (Hwk : Δ |-* T : K) :=
   match n with
     | O => T
     | S n' => 
         match step_dec T Δ K Hwk with
         | inl (existT _ T' P) => 
             let Hwk' := @step_preserves_kinding T T' Δ K Hwk P in
-            normaliser_gas n' Hwk'
+            normalizer_gas n' Hwk'
         | inr _ => T
         end
   end.
 
-Definition normaliser_wk {T Δ K} (Hwk : Δ |-* T : K) : ty :=
-  let HSN := plutus_ty_strong_normalization T Δ K Hwk in
+(* Return for any well-typed input a normal form *)
+Definition normalizer_wk {T Δ K} (Hwk : Δ |-* T : K) : ty :=
+  let HSN := strong_normalization_PIR T Δ K Hwk in
   projT1 (SN_normalise T Δ K Hwk HSN).
 
-Definition normaliser Δ T : option ty :=
+(* The normalizer procedure *)
+Definition normalizer Δ T : option ty :=
   match kind_check Δ T with
   | Some K => fun Hkc =>
-      Some (normaliser_wk (kind_checking_sound Δ T K Hkc))
+      Some (normalizer_wk (kind_checking_sound Δ T K Hkc))
   | None => fun _ => None
   end eq_refl.
 
-Theorem normaliser__well_kinded Δ T Tn :
-  normaliser Δ T = Some Tn -> {K & Δ |-* T : K}.
+(* The normalizer only returns a normal form for well-kinded types *)
+Theorem normalizer__well_kinded Δ T Tn :
+  normalizer Δ T = Some Tn -> {K & Δ |-* T : K}.
 Proof.
-  unfold normaliser.
+  unfold normalizer.
   move: eq_refl.
   case: {2 3}(kind_check Δ T) => // a e H. (* TODO: I don't understand (all of) this ssreflect stuff, see https://stackoverflow.com/questions/47345174/using-destruct-on-pattern-match-expression-with-convoy-pattern*)
   inversion H.
@@ -83,17 +86,21 @@ Proof.
   now apply kind_checking_sound.
 Qed.
 
-Fixpoint map_normaliser (xs : list (string * ty * (list (string * kind)))) :=
+(* Normalise multiple types in a list.
+  Each element in the list is a tuple (X, T Δ) where X is a name, T a type, and Δ the context for which we normalise T.
+*)
+Fixpoint map_normalizer (xs : list (string * ty * (list (string * kind)))) :=
   match xs with
   | nil => Some nil
-  | ((X, T, Δ) :: xs') => normaliser Δ T >>= fun Tn => 
-                     map_normaliser xs' >>= fun xs'' =>
+  | ((X, T, Δ) :: xs') => normalizer Δ T >>= fun Tn => 
+                     map_normalizer xs' >>= fun xs'' =>
                      Some ((X, Tn) ::xs'')
   end.
 
-Lemma map_normaliser_unfold {Δ : list (string * kind)} {X T} {xs xs'} :
-  map_normaliser ((X, T, Δ) :: xs) = Some xs'
-  -> exists Tn xs'', (xs' = (X, Tn)::xs'') /\ normaliser Δ T = Some Tn /\ (map_normaliser xs = Some xs'').
+(* If a list map_normalises, then the first element also normalises *)
+Lemma map_normalizer_unfold {Δ : list (string * kind)} {X T} {xs xs'} :
+  map_normalizer ((X, T, Δ) :: xs) = Some xs'
+  -> exists Tn xs'', (xs' = (X, Tn)::xs'') /\ normalizer Δ T = Some Tn /\ (map_normalizer xs = Some xs'').
 Proof.
   intros.
   inversion H.
@@ -105,8 +112,9 @@ Proof.
   auto.
 Qed.
 
-Lemma map_normaliser__well_kinded xs xs' :
-  map_normaliser xs = Some xs' -> map_wk xs.
+(* normalizer__well_kinded for multiple types *)
+Lemma map_normalizer__well_kinded xs xs' :
+  map_normalizer xs = Some xs' -> map_wk xs.
 Proof.
   intros.
   generalize dependent xs'.
@@ -114,9 +122,9 @@ Proof.
   - inversion H; subst.
     constructor.
   - destruct a as [[X T] Δ].
-    apply map_normaliser_unfold in H.
+    apply map_normalizer_unfold in H.
     destruct H as [Tn [xs'' [Heq [Hnorm Hmap]] ] ].
-    apply normaliser__well_kinded in Hnorm as [K Hwk].
+    apply normalizer__well_kinded in Hnorm as [K Hwk].
     apply MW_cons with (K := K).
     + apply (IHxs xs''); auto.
     + assumption.
