src/Language/STLC/Alpha/alpha.v
@@ -1181,3 +1181,26 @@ Proof.
     + eauto.
     + apply alpha_extend_ids. apply ctx_id_right_is_id. eauto.
 Qed.
+
+Create HintDb α_eq_db.
+Hint Constructors Alpha : α_eq_db.
+Hint Resolve alpha_refl : α_eq_db.
+Hint Resolve alpha_sym : α_eq_db.
+Hint Resolve alpha_trans : α_eq_db.
+Hint Constructors AlphaVar : α_eq_db.
+Hint Constructors AlphaCtxSym : α_eq_db.
+Hint Constructors αCtxTrans : α_eq_db.
+Hint Resolve alpha_extend_ids : α_eq_db.
+Hint Constructors IdCtx : α_eq_db.
+Hint Resolve sym_alpha_ctx_is_sym : α_eq_db.
+Hint Resolve sym_alpha_ctx_is_sym : α_eq_db.
+Hint Resolve sym_alpha_ctx_left_is_sym  : α_eq_db.
+Hint Constructors LegalRenSwap : α_eq_db.
+Hint Unfold LegalRenSwaps : α_eq_db.
+
+Create HintDb α_eq_db_trans.
+Hint Resolve id_left_trans : α_eq_db_trans.
+Hint Resolve id_right_trans : α_eq_db_trans.
+Hint Resolve alpha_extend_ids : α_eq_db_trans.
+Hint Resolve ctx_id_left_is_id : α_eq_db_trans.
+Hint Resolve ctx_id_right_is_id : α_eq_db_trans.
