src/PlutusIR/Semantics/Static/Normalization/Normalizer_sound_complete.v
@@ -1,34 +1,37 @@
 From PlutusCert Require Import 
   PlutusIR 
-  Normalisation.BigStep 
+  Normalization.BigStep 
   Kinding.Kinding
   Kinding.Checker
-  Normalisation.SmallStep
+  Normalization.SmallStep
   Util
   SubstituteTCA
   SN_PIR
-  Normaliser
-  Normalisation.Preservation
+  Normalizer
+  Normalization.Preservation
   .
 Require Import Coq.Lists.List.
 Import ListNotations.
 Require Import Coq.Strings.String.
+Require Import Coq.Program.Equality.
 
+(* Dependently typed version: Normalization is sound for well-kinded types *)
 Theorem norm_sound Tn {T Δ K} (Hwk : Δ |-* T : K) :
-  normaliser_wk Hwk = Tn -> normalise T Tn.
+  normalizer_wk Hwk = Tn -> normalise T Tn.
 Proof.
   intros.
-  unfold normaliser_wk in H.
+  unfold normalizer_wk in H.
   destruct SN_normalise in H; eauto.
   subst.
   assumption.
 Qed.
 
+(* Dependently typed version: Normalization is complete for well-kinded types *)
 Theorem norm_complete Δ K (T Tn : ty) (Hwk : Δ |-* T : K):
-  normalise T Tn -> normaliser_wk Hwk = Tn.
+  normalise T Tn -> normalizer_wk Hwk = Tn.
 Proof.
   intros HnormR.
-  unfold normaliser_wk.
+  unfold normalizer_wk.
   destruct SN_normalise.
   simpl.
   now apply (normalisation__deterministic T x Tn) in n.
@@ -36,27 +39,23 @@ Qed.
 
 From Coq Require Import ssreflect.
 
-Theorem normaliser_sound Δ T Tn :
-  normaliser Δ T = Some Tn -> normalise T Tn.
+(* The normalizer is sound for well-kinded types*)
+Theorem normalizer_sound Δ T Tn :
+  normalizer Δ T = Some Tn -> normalise T Tn.
 Proof.
-  unfold normaliser.
+  unfold normalizer.
   move: eq_refl.
   case: {2 3}(kind_check Δ T) => // a e H. (* TODO: I don't understand (all of) this ssreflect stuff, see https://stackoverflow.com/questions/47345174/using-destruct-on-pattern-match-expression-with-convoy-pattern*)
   inversion H.
   eapply norm_sound; eauto.
 Qed.
 
-(* We need the well-kinded assumption, otherwise counterexample:
-    nil |-* TyApp (Lam bX Kind_Base "bX") (Lam bY Kind_Base "bY")
-
-    which normalises to Lam bY Kind_Base "bY",
-    but normaliser _ T will return None
-
+(* The normalizer is complete for well-kinded types
 *)
-Theorem normaliser_complete {K Δ T Tn} :
-  Δ |-* T : K -> normalise T Tn -> normaliser Δ T = Some Tn.
+Theorem normalizer_complete {K Δ T Tn} :
+  Δ |-* T : K -> normalise T Tn -> normalizer Δ T = Some Tn.
 Proof.
-  unfold normaliser.
+  unfold normalizer.
   intros.
   apply kind_checking_complete in H.
   move: eq_refl.
@@ -69,12 +68,14 @@ Proof.
     discriminate.
 Qed.
 
+(* Remove kinding contexts from a triple *)
 Fixpoint remove_deltas  {A B C : Type} (xs : list (A * B * C)) :=
   match xs with
   | nil => nil 
   | (X, T, _) :: xs' => (X, T) :: (remove_deltas xs')
   end.
 
+(* Remove_deltas distributes *)
 Lemma remove_deltas_app {A B C : Type} (xs ys : list (A * B * C)) :
   remove_deltas (xs ++ ys) = remove_deltas xs ++ remove_deltas ys.
 Proof.
@@ -87,9 +88,9 @@ Proof.
     reflexivity.
 Qed.
     
-
-Lemma map_normaliser_sound xs xs' :
-  map_normaliser xs = Some xs' -> map_normalise (remove_deltas xs) xs'.
+(* Normalization sound for list of (X, T, Δ) triples*)
+Lemma map_normalizer_sound xs xs' :
+  map_normalizer xs = Some xs' -> map_normalise (remove_deltas xs) xs'.
 Proof.
   intros.
   generalize dependent xs'.
@@ -97,19 +98,17 @@ Proof.
   - inversion H; subst.
     constructor.
   - destruct a as [[X T] Δ].
-    apply map_normaliser_unfold in H.
+    apply map_normalizer_unfold in H.
     destruct H as [Tn [xs'' [Heq [Hnorm Hmap]] ] ].
     rewrite Heq.
     constructor.
     + now apply IHxs.
-    + eapply normaliser_sound; eauto.
+    + eapply normalizer_sound; eauto.
 Qed.
 
-Require Import Coq.Program.Equality.
-
-(* Basically we need a map_wellkinded argument *)
-Lemma map_normaliser_complete {xs : list (string * ty * (list (string * kind)))} {xs'} :
-  map_wk xs -> map_normalise (remove_deltas xs) xs' -> map_normaliser xs = Some xs'.
+(* map_normalizer complete for well-kinded types *)
+Lemma map_normalizer_complete {xs : list (string * ty * (list (string * kind)))} {xs'} :
+  map_wk xs -> map_normalise (remove_deltas xs) xs' -> map_normalizer xs = Some xs'.
 Proof.
   intros.
   dependent induction H0.
@@ -145,7 +144,7 @@ Proof.
         reflexivity.
       }
       subst.
-      apply (normaliser_complete H3) in H1.
+      apply (normalizer_complete H3) in H1.
       specialize (IHmap_normalise xs0 H2).
       assert (Ts = remove_deltas xs0).
       {
@@ -154,10 +153,10 @@ Proof.
         auto.
       }
       specialize (IHmap_normalise H4).
-      unfold map_normaliser.
+      unfold map_normalizer.
       rewrite H1.
       simpl.
-      fold map_normaliser.
+      fold map_normalizer.
       rewrite IHmap_normalise.
       simpl.
       assert (X = X0).
@@ -171,11 +170,11 @@ Proof.
       reflexivity.
 Qed.
 
-
-Theorem normaliser_preserves_kinding {Δ T Tn K } :
-  Δ |-* T : K -> normaliser Δ T = Some Tn -> Δ |-* Tn : K.
+(* The normalizer preserves kinding *)
+Theorem normalizer_preserves_kinding {Δ T Tn K } :
+  Δ |-* T : K -> normalizer Δ T = Some Tn -> Δ |-* Tn : K.
 Proof.
   intros.
-  apply (normaliser_sound) in H0.
+  apply (normalizer_sound) in H0.
   apply (normalisation_preserves_kinding H) in H0; auto.
 Qed.
