src/PlutusIR/Semantics/Static/Typing/Typechecker.v
@@ -7,9 +7,9 @@ Require Import Coq.Strings.String.
 Local Open Scope string_scope.
 
 From PlutusCert Require Import 
-    Normalisation.BigStep
-    Normalisation.Normaliser_sound_complete
-    Normalisation.Normaliser
+    Normalization.BigStep
+    Normalization.Normalizer_sound_complete
+    Normalization.Normalizer
     PlutusIR 
     Static.Typing.Typing
     Util.List
@@ -24,28 +24,29 @@ Require Import PlutusCert.PlutusIR.Analysis.BoundVars.
 
 From Coq Require Import Program.Equality.
 
-(* Find instead of in_dec for performance?*)
+(* Procedure that checks for no duplicate keys *)
 Fixpoint no_dup_fun (xs : list string) := 
   match xs with
   | nil => true
   | (x::xs) => if in_dec string_dec x xs then false else no_dup_fun xs
   end.
 
-
+(* Helper that returns if the kind is * *)
 Definition is_KindBase (k : option kind) : bool :=
   match k with 
   | Some Kind_Base => true
   | _ => false
   end.
 
+(* Procedure for well-formed constructures *)
 Definition constructor_well_formed_check (Δ : list (binderTyname * kind)) (v : vdecl) (Tr : ty ) : bool :=
   match v with
   | VarDecl x T => let (targs, tr') := splitTy T in
           Ty_eqb Tr tr' && forallb (fun U => is_KindBase (kind_check Δ U)) targs
   end.
 
-(* Idea Jacco: pass the recursively called type_check function as an argument even though it is not defined yet 
-Make another version that already has type_check as argument after type_check is defined.
+(* Procedure for determining whether a binding is well-formed. *)
+(* Pass the recursively called type_check function as an argument even though it is not defined yet.
 *)
 Definition binding_well_formed_check 
   (type_check' : ((list (binderTyname * kind)) -> (list (binderName * ty)) -> term -> option ty)) 
@@ -58,7 +59,7 @@ Definition binding_well_formed_check
     | (TermBind s (VarDecl x T) t) => match kind_check Δ T with
                                       | Some Kind_Base => 
                                         match type_check' Δ Γ t with   
-                                        | Some Tn => match normaliser Δ T with
+                                        | Some Tn => match normalizer Δ T with
                                                     | Some Tn' => Ty_eqb Tn Tn'
                                                     | _ => false
                                                     end
@@ -92,7 +93,8 @@ Definition binding_well_formed_check
       else false
     end.
 
-(* first argument represents binding_well_formed with the type_check already passed in *)
+(* Procedure for checking well-formedness of non-recursive lists of bindings *)
+(* first argument represents binding_well_formed with the type_check function already passed in *)
 Definition bindings_well_formed_nonrec_check : 
   ((list (binderTyname * kind)) -> (list (binderName * ty)) -> recursivity -> binding -> bool) ->
   list (binderTyname * kind) -> (list (binderName * ty)) -> (list binding) -> bool :=
@@ -100,7 +102,7 @@ Definition bindings_well_formed_nonrec_check :
   fix f Δ Γ bs :=
     match bs with
       | (b::bs') =>
-            match (map_normaliser (insert_deltas_rec (binds_Gamma b) (binds_Delta b ++ Δ))) with
+            match (map_normalizer (insert_deltas_rec (binds_Gamma b) (binds_Delta b ++ Δ))) with
             | Some bsGn =>
               b_wf Δ Γ NonRec b && f ((binds_Delta b) ++ Δ) (bsGn ++ Γ) bs'
             | _ => false
@@ -108,6 +110,7 @@ Definition bindings_well_formed_nonrec_check :
       | _ => true
     end.
 
+(* Procedure for checking well-formedness of recursive lists of bindings *)
 Definition bindings_well_formed_rec_check : (binding -> bool) -> list binding -> bool :=
   fun b_wf =>
   fix f bs :=
@@ -116,15 +119,17 @@ Definition bindings_well_formed_rec_check : (binding -> bool) -> list binding ->
       | _ => true
     end.
 
+(* Procedure for checking the type of a term. *)
+(* Uses normalization and kind_check procedures *)
 Fixpoint type_check (Δ : list (binderTyname * kind)) (Γ : list (binderName * ty)) (term : term) {struct term} : (option ty) :=
     match term with
     | Var x => lookup x Γ >>= fun T => 
                 match kind_check Δ T with
-                | Some Kind_Base => normaliser Δ T
+                | Some Kind_Base => normalizer Δ T
                 | _ => None
                 end
     | LamAbs x T1 t => 
-        normaliser Δ T1 >>= fun T1n =>
+        normalizer Δ T1 >>= fun T1n =>
         match type_check Δ ((x, T1n) :: Γ) t, kind_check Δ T1 with
         | Some T2, Some Kind_Base => Some (Ty_Fun T1n T2) 
         | _, _ => None
@@ -144,8 +149,8 @@ Fixpoint type_check (Δ : list (binderTyname * kind)) (Γ : list (binderName * t
         match type_check Δ Γ t1, kind_check Δ T2 with
         | Some (Ty_Forall X K2 T1), Some K2' =>
             if Kind_eqb K2 K2' then 
-                normaliser Δ T2 >>= fun T2n =>
-                normaliser Δ (substituteTCA X T2n T1) >>= fun T0n =>
+                normalizer Δ T2 >>= fun T2n =>
+                normalizer Δ (substituteTCA X T2n T1) >>= fun T0n =>
                 Some T0n
             else None
         | _, _ => None
@@ -154,9 +159,9 @@ Fixpoint type_check (Δ : list (binderTyname * kind)) (Γ : list (binderName * t
         match kind_check Δ T, kind_check Δ F, type_check Δ Γ M with
         | Some K, Some (Kind_Arrow (Kind_Arrow K' Kind_Base) (Kind_Arrow K'' Kind_Base)), Some T0n
             => if andb (Kind_eqb K K') (Kind_eqb K K'') then
-                    normaliser Δ T >>= fun Tn =>
-                    normaliser Δ F >>= fun Fn =>
-                    normaliser Δ (unwrapIFix Fn K Tn) >>= fun T0n' =>
+                    normalizer Δ T >>= fun Tn =>
+                    normalizer Δ F >>= fun Fn =>
+                    normalizer Δ (unwrapIFix Fn K Tn) >>= fun T0n' =>
                     if Ty_eqb T0n T0n' then 
                         Some (Ty_IFix Fn Tn)
                     else None 
@@ -168,7 +173,7 @@ Fixpoint type_check (Δ : list (binderTyname * kind)) (Γ : list (binderName * t
             | Some (Ty_IFix F T) =>
                 match kind_check Δ T with
                     | Some K =>
-                          normaliser Δ (unwrapIFix F K T) >>= fun T0n => Some T0n
+                          normalizer Δ (unwrapIFix F K T) >>= fun T0n => Some T0n
                         
                     | _  => None
                     end 
@@ -177,16 +182,16 @@ Fixpoint type_check (Δ : list (binderTyname * kind)) (Γ : list (binderName * t
     | Constant (ValueOf T a) => Some (Ty_Builtin T)
     | Builtin f =>
         let T := lookupBuiltinTy f in
-        normaliser Δ T >>= fun Tn =>
+        normalizer Δ T >>= fun Tn =>
         Some Tn
-    | Error S' => normaliser Δ S' >>= fun S'n => match kind_check Δ S' with
+    | Error S' => normalizer Δ S' >>= fun S'n => match kind_check Δ S' with
         | Some Kind_Base => Some S'n
         | _ => None
         end
     | Let NonRec bs t =>
         let Δ' := flatten (map binds_Delta bs) ++ Δ in
         let xs := (insert_deltas_bind_Gamma_nr bs Δ) in
-          map_normaliser xs >>= fun bsgn => 
+          map_normalizer xs >>= fun bsgn => 
           let Γ' := bsgn ++ Γ in
           if (bindings_well_formed_nonrec_check (binding_well_formed_check type_check) Δ Γ bs) then 
             type_check Δ' Γ' t >>= fun T =>
@@ -200,7 +205,7 @@ Fixpoint type_check (Δ : list (binderTyname * kind)) (Γ : list (binderName * t
         if no_dup_fun (btvbs bs) && no_dup_fun (bvbs bs) then
           let Δ' := flatten (map binds_Delta bs) ++ Δ in
           let xs := (insert_deltas_rec (flatten (map binds_Gamma bs)) Δ') in
-            map_normaliser xs >>= fun bsgn =>
+            map_normalizer xs >>= fun bsgn =>
             let Γ' := bsgn ++ Γ in
               if (bindings_well_formed_rec_check (binding_well_formed_check type_check Δ' Γ' Rec) bs) then 
                 type_check Δ' Γ' t >>= fun T =>
@@ -211,5 +216,5 @@ Fixpoint type_check (Δ : list (binderTyname * kind)) (Γ : list (binderName * t
                     end 
               else None
           else None
-    | _ => None (* TODO: Case and Constr?? *)
+    | _ => None (* TODO: Case and Constr. Also not defined in the relation yet. *)
     end.
