src/PlutusIR/Semantics/Static/Typing/drop_context.v
@@ -17,9 +17,11 @@ Import ListNotations.
 Import Coq.Strings.String.
 Local Open Scope string_scope.
 Open Scope list_scope.
+From Coq Require Import Bool.
 
 (* ************* drop_ty_var ************* *)
 
+(* Using drop_ty_var creates a smaller list in the sense of inclusion *)
 Lemma drop_ty_var__inclusion X Γ :
   List.inclusion (drop_ty_var X Γ) Γ.
 Proof.
@@ -33,7 +35,8 @@ Proof.
     destruct (string_dec a1 x); subst.
     + rewrite String.eqb_refl.
       f_equal.
-      (* Suppose X in a2. Then by Hl
+      (* ADMITTED: 
+        Suppose X in a2. Then by Hl
         we have that a2 <> v
 
         But then by drop_ty_var, all keys "x" will be removed from Hl,
@@ -45,15 +48,18 @@ Proof.
       admit.
     + rewrite <- String.eqb_neq in n.
       rewrite n.
-      (* a1 <> x
+      (* ADMITTED: 
+        a1 <> x
         lookup x (drop ((a1, a2)::Γ) = Some v)
         Well, it is not the first one (a1), and the result is Some v.
         Hence we must have lookup x (drop Γ) = Some v. (possibly with even smaller Gamma, if a2 contains X)
         since drop Γ is a subset of Γ, we must have then also lookup x Γ = Some v.
       *)
+      admit.
 
 Admitted.
 
+(* Drop_ty_var preserves inclusion *)
 Lemma drop_ty_var__inclusion_preserving : forall X Γ Γ',
     List.inclusion Γ Γ' -> List.inclusion (drop_ty_var X Γ) (drop_ty_var X Γ').
 Proof.
@@ -78,6 +84,7 @@ intros x v Hl.
 *)
 Admitted.
 
+(* If x is present after drop_ty_var, then it was also present before drop_ty_var *)
 Lemma drop_ty_var__lookup_some : forall X Γ x T,
     lookup x (drop_ty_var X Γ) = Some T ->
     exists T', lookup x Γ = Some T'.
@@ -88,6 +95,7 @@ Admitted.
 
 (* Drop Δ *)
 
+(* Dropping nothing is identity *)
 Lemma drop_Δ_nil : forall Δ,
     drop_Δ Δ nil = Δ.
 Proof.
@@ -99,8 +107,7 @@ Proof.
     auto.
 Qed.
 
-From Coq Require Import Bool.
-
+(* All elements in bind_Delta b are dropped by drop_Δ _ b... *)
 Lemma drop_Δ__weaken : forall Δ b bs,
   drop_Δ Δ (b::bs) = drop_Δ (binds_Delta b ++ Δ) (b::bs).
 Proof.
@@ -155,6 +162,7 @@ Proof.
 Qed.
 
 
+(* drop_Δ with multiple bindings can be unfolded *)
 Lemma drop_Δ__unfold : forall Δ b bs,
   drop_Δ Δ (b::bs) = drop_Δ (drop_Δ Δ bs) [b].
 Proof.
@@ -218,6 +226,7 @@ Proof.
       apply IHΔ.
 Qed.
 
+(* Trivial helper: Drop_Δ nil preserves kinding (and is identical)*)
 Lemma drop_Δ_nil__kinding : forall Δ T K,
     drop_Δ Δ nil |-* T : K -> Δ |-* T : K.
 Proof.
@@ -226,166 +235,176 @@ Proof.
   assumption.
 Qed.
     
-  Lemma drop_Δ'__lookup_None : forall Δ xs x,
-    In x (xs) -> lookup x (drop_Δ' Δ xs) = None.
-  Proof.
-    intros Δ xs x Hbtvbs.
-    induction Δ; simpl.
-    - reflexivity.
-    - destruct a as [a1 a2]; simpl.
-      destruct (negb (inb_string a1 (xs))) eqn:Heqn.
-      + destruct (string_dec a1 x).
-        * subst.
-          exfalso.
-          rewrite negb_true_iff in Heqn.
-          rewrite inb_string_false_iff in Heqn.
-          contradiction.
-        * simpl.
-          rewrite <- String.eqb_neq in n.
-          rewrite n.
-          exact IHΔ.
-    + assumption.
-  Qed.
+(* drop_Δ' drops everything in the list *)
+Lemma drop_Δ'__lookup_None : forall Δ xs x,
+  In x (xs) -> lookup x (drop_Δ' Δ xs) = None.
+Proof.
+  intros Δ xs x Hbtvbs.
+  induction Δ; simpl.
+  - reflexivity.
+  - destruct a as [a1 a2]; simpl.
+    destruct (negb (inb_string a1 (xs))) eqn:Heqn.
+    + destruct (string_dec a1 x).
+      * subst.
+        exfalso.
+        rewrite negb_true_iff in Heqn.
+        rewrite inb_string_false_iff in Heqn.
+        contradiction.
+      * simpl.
+        rewrite <- String.eqb_neq in n.
+        rewrite n.
+        exact IHΔ.
+  + assumption.
+Qed.
 
-  Lemma drop_Δ__lookup_None : forall Δ bs x,
-    In x (BoundVars.btvbs bs) -> lookup x (drop_Δ Δ bs) = None.
-  Proof.
-    intros.
-    unfold drop_Δ.
-    eapply drop_Δ'__lookup_None.
-    assumption.
-  Qed.
+(* drop_Δ drops all introduced binder names *)
+Lemma drop_Δ__lookup_None : forall Δ bs x,
+  In x (BoundVars.btvbs bs) -> lookup x (drop_Δ Δ bs) = None.
+Proof.
+  intros.
+  unfold drop_Δ.
+  eapply drop_Δ'__lookup_None.
+  assumption.
+Qed.
 
-  Lemma dropped_not_in_drop_Δ' : forall Δ xs x,
-    In x xs ->
-    ~ In x (map fst (drop_Δ' Δ xs)).
-  Proof.
-    intros Δ xs x Hin.
-    apply drop_Δ'__lookup_None with (Δ := Δ) in Hin.
-    apply lookup__not_in in Hin.
-    assumption.
-  Qed.
+(* drop_Δ'__lookup_None, but for In instead of lookup*)
+Lemma dropped_not_in_drop_Δ' : forall Δ xs x,
+  In x xs ->
+  ~ In x (map fst (drop_Δ' Δ xs)).
+Proof.
+  intros Δ xs x Hin.
+  apply drop_Δ'__lookup_None with (Δ := Δ) in Hin.
+  apply lookup__not_in in Hin.
+  assumption.
+Qed.
 
-   Lemma lookup_None__drop_Δ' : forall Δ xs x,
-    ~ In x xs ->
-    lookup x (drop_Δ' Δ xs) = lookup x Δ.
-  Proof.
-    intros Δ xs x HnotBtvb.
-    induction Δ; simpl.
-    - reflexivity.
-    - destruct a as [a1 a2]; simpl.
-      destruct ((inb_string a1 xs)) eqn:Heqn; simpl.
-      + destruct (string_dec a1 x).
-        * subst.
-          rewrite inb_string_true_iff in Heqn.
-          contradiction.
-        * rewrite <- String.eqb_neq in n.
-          rewrite n.
-          rewrite IHΔ; auto.
-      + simpl.
-        destruct (string_dec a1 x).
-        * subst.
-          rewrite String.eqb_refl.
-          reflexivity.
-        * rewrite <- String.eqb_neq in n.
-          rewrite n.
-          rewrite IHΔ; auto. 
-  Qed.
+(* drop_Δ' does not drop anything not in xs *)
+Lemma lookup_None__drop_Δ' : forall Δ xs x,
+  ~ In x xs ->
+  lookup x (drop_Δ' Δ xs) = lookup x Δ.
+Proof.
+  intros Δ xs x HnotBtvb.
+  induction Δ; simpl.
+  - reflexivity.
+  - destruct a as [a1 a2]; simpl.
+    destruct ((inb_string a1 xs)) eqn:Heqn; simpl.
+    + destruct (string_dec a1 x).
+      * subst.
+        rewrite inb_string_true_iff in Heqn.
+        contradiction.
+      * rewrite <- String.eqb_neq in n.
+        rewrite n.
+        rewrite IHΔ; auto.
+    + simpl.
+      destruct (string_dec a1 x).
+      * subst.
+        rewrite String.eqb_refl.
+        reflexivity.
+      * rewrite <- String.eqb_neq in n.
+        rewrite n.
+        rewrite IHΔ; auto. 
+Qed.
 
-  Lemma lookup_None__drop_Δ : forall Δ bs x,
-    ~ In x (BoundVars.btvbs bs) ->
-    lookup x (drop_Δ Δ bs) = lookup x Δ.
-  Proof.
-    intros.
-    unfold drop_Δ.
-    eapply lookup_None__drop_Δ'.
-    assumption.
-  Qed.
+(* drop_Δ only drops introduced binders *)
+Lemma lookup_None__drop_Δ : forall Δ bs x,
+  ~ In x (BoundVars.btvbs bs) ->
+  lookup x (drop_Δ Δ bs) = lookup x Δ.
+Proof.
+  intros.
+  unfold drop_Δ.
+  eapply lookup_None__drop_Δ'.
+  assumption.
+Qed.
 
-  Lemma lookup_Some__drop_Δ'_no_xs : forall Δ xs x K,
-    lookup x (drop_Δ' Δ xs) = Some K ->
-    ~ In x xs.
-  Proof.
-    intros Δ xs x K Hl.
-    induction Δ; simpl in *.
-    - inversion Hl.
-    - destruct a as [a1 a2]; simpl in *.
-      destruct (inb_string a1 xs) eqn:Heqn; simpl in *.
-      + destruct (string_dec a1 x).
-        * apply IHΔ.
-          assumption.
-        * subst.
-          apply IHΔ.
-          exact Hl.
-      + simpl in Hl.
-        destruct (string_dec a1 x).
-        * subst.
-          rewrite inb_string_false_iff in Heqn.
-          assumption.
-        * rewrite <- String.eqb_neq in n.
-          rewrite n in Hl.
-          apply IHΔ.
-          assumption.
-  Qed.
+(* If lookup finds something after drop_Δ', then it cannot be in the list xs that should have been dropped *)
+Lemma lookup_Some__drop_Δ'_no_xs : forall Δ xs x K,
+  lookup x (drop_Δ' Δ xs) = Some K ->
+  ~ In x xs.
+Proof.
+  intros Δ xs x K Hl.
+  induction Δ; simpl in *.
+  - inversion Hl.
+  - destruct a as [a1 a2]; simpl in *.
+    destruct (inb_string a1 xs) eqn:Heqn; simpl in *.
+    + destruct (string_dec a1 x).
+      * apply IHΔ.
+        assumption.
+      * subst.
+        apply IHΔ.
+        exact Hl.
+    + simpl in Hl.
+      destruct (string_dec a1 x).
+      * subst.
+        rewrite inb_string_false_iff in Heqn.
+        assumption.
+      * rewrite <- String.eqb_neq in n.
+        rewrite n in Hl.
+        apply IHΔ.
+        assumption.
+Qed.
 
-  Lemma lookup_Some__drop_Δ_no_btvbs : forall Δ bs x K,
-    lookup x (drop_Δ Δ bs) = Some K ->
-    ~ In x (BoundVars.btvbs bs).
-  Proof.
-    intros.
-    unfold drop_Δ.
-    eapply lookup_Some__drop_Δ'_no_xs; eauto.
-  Qed.
+(* Analogous but for drop_Δ*)
+Lemma lookup_Some__drop_Δ_no_btvbs : forall Δ bs x K,
+  lookup x (drop_Δ Δ bs) = Some K ->
+  ~ In x (BoundVars.btvbs bs).
+Proof.
+  intros.
+  unfold drop_Δ.
+  eapply lookup_Some__drop_Δ'_no_xs; eauto.
+Qed.
 
-  Lemma drop_Δ'__inclusion : forall Δ xs,
-    List.inclusion (drop_Δ' Δ xs) Δ.
-  Proof.
-    intros.
-    induction Δ; simpl.
-    - unfold List.inclusion; auto.
-    - destruct a as [a1 a2].
-      destruct (inb_string (fst (a1, a2)) xs) eqn:Heqn; simpl in *.
-      + unfold inclusion.
-        intros x v Hl.
-        destruct (string_dec a1 x).
-        * subst.
-          exfalso.
-          rewrite inb_string_true_iff in Heqn.
-          eapply drop_Δ'__lookup_None in Heqn.
-          rewrite Hl in Heqn.
-          inversion Heqn.
-        * simpl.
-          rewrite <- String.eqb_neq in n.
-          rewrite n.
-          apply IHΔ.
-          assumption.
-      + unfold inclusion.
-        intros x v Hl.
-        destruct (string_dec a1 x).
-        * subst.
-          inversion Hl.
-          rewrite String.eqb_refl.
-          simpl.
-          rewrite String.eqb_refl.
-          reflexivity.
-        * simpl.
-          rewrite <- String.eqb_neq in n.
-          rewrite n.
-          apply IHΔ.
-          simpl in Hl.
-          rewrite n in Hl.
-          assumption.
-  Qed.
+(* drop_Δ' is included in Δ*)
+Lemma drop_Δ'__inclusion : forall Δ xs,
+  List.inclusion (drop_Δ' Δ xs) Δ.
+Proof.
+  intros.
+  induction Δ; simpl.
+  - unfold List.inclusion; auto.
+  - destruct a as [a1 a2].
+    destruct (inb_string (fst (a1, a2)) xs) eqn:Heqn; simpl in *.
+    + unfold inclusion.
+      intros x v Hl.
+      destruct (string_dec a1 x).
+      * subst.
+        exfalso.
+        rewrite inb_string_true_iff in Heqn.
+        eapply drop_Δ'__lookup_None in Heqn.
+        rewrite Hl in Heqn.
+        inversion Heqn.
+      * simpl.
+        rewrite <- String.eqb_neq in n.
+        rewrite n.
+        apply IHΔ.
+        assumption.
+    + unfold inclusion.
+      intros x v Hl.
+      destruct (string_dec a1 x).
+      * subst.
+        inversion Hl.
+        rewrite String.eqb_refl.
+        simpl.
+        rewrite String.eqb_refl.
+        reflexivity.
+      * simpl.
+        rewrite <- String.eqb_neq in n.
+        rewrite n.
+        apply IHΔ.
+        simpl in Hl.
+        rewrite n in Hl.
+        assumption.
+Qed.
 
-  Lemma drop_Δ__inclusion : forall Δ bs,
-    List.inclusion (drop_Δ Δ bs) Δ.
-  Proof.
-    intros.
-    unfold drop_Δ.
-    eapply drop_Δ'__inclusion.
-  Qed.
+(* drop_Δ is included in Δ*)
+Lemma drop_Δ__inclusion : forall Δ bs,
+  List.inclusion (drop_Δ Δ bs) Δ.
+Proof.
+  intros.
+  unfold drop_Δ.
+  eapply drop_Δ'__inclusion.
+Qed.
 
 
+(* Not removing b and adding them to Δ is a superset *)
 Lemma drop_Δ_cons__inclusion : forall Δ b bs,
     List.inclusion (drop_Δ Δ (b::bs)) (drop_Δ (binds_Delta b ++ Δ) bs).
 Proof.
@@ -403,41 +422,44 @@ Proof.
   apply drop_Δ__inclusion.
 Qed.
 
-  Lemma drop_Δ'__preserves__inclusion : forall Δ Δ' xs,
-      List.inclusion Δ Δ' ->
-      List.inclusion (drop_Δ' Δ xs) (drop_Δ' Δ' xs).
-  Proof.
-    intros Δ Δ' xs Hincl.
-    unfold inclusion in *.
-    intros x v Hl.
-    assert (lookup x Δ' = Some v).
-    {
-      apply drop_Δ'__inclusion in Hl.
-      apply Hincl in Hl.
-      assumption.
-    }
-    assert ( ~ In x xs).
-    {
-      eapply lookup_Some__drop_Δ'_no_xs; eauto.
-    }
-
-    induction Δ'.
-    - inversion H.
-    - eapply lookup_None__drop_Δ' in H0; eauto.
-      rewrite H0.
-      assumption.
-  Qed.
-
-  Lemma drop_Δ__preserves__inclusion : forall Δ Δ' bs,
-      List.inclusion Δ Δ' ->
-      List.inclusion (drop_Δ Δ bs) (drop_Δ Δ' bs).
-  Proof.
-    intros.
-    unfold drop_Δ.
-    eapply drop_Δ'__preserves__inclusion.
+(* drop_Δ' prserves inclusion *)
+Lemma drop_Δ'__preserves__inclusion : forall Δ Δ' xs,
+    List.inclusion Δ Δ' ->
+    List.inclusion (drop_Δ' Δ xs) (drop_Δ' Δ' xs).
+Proof.
+  intros Δ Δ' xs Hincl.
+  unfold inclusion in *.
+  intros x v Hl.
+  assert (lookup x Δ' = Some v).
+  {
+    apply drop_Δ'__inclusion in Hl.
+    apply Hincl in Hl.
     assumption.
-  Qed.
+  }
+  assert ( ~ In x xs).
+  {
+    eapply lookup_Some__drop_Δ'_no_xs; eauto.
+  }
 
+  induction Δ'.
+  - inversion H.
+  - eapply lookup_None__drop_Δ' in H0; eauto.
+    rewrite H0.
+    assumption.
+Qed.
+
+(* drop_Δ preserves inclusion *)
+Lemma drop_Δ__preserves__inclusion : forall Δ Δ' bs,
+    List.inclusion Δ Δ' ->
+    List.inclusion (drop_Δ Δ bs) (drop_Δ Δ' bs).
+Proof.
+  intros.
+  unfold drop_Δ.
+  eapply drop_Δ'__preserves__inclusion.
+  assumption.
+Qed.
+
+(* If the bound type variables in two lists of bindings are identical, then drop_Δ behaviour is too *)
 Lemma btvbs_eq__drop_Δ_eq : forall Δ bs bs',
   btvbs bs = btvbs bs' ->
   drop_Δ Δ bs = drop_Δ Δ bs'.
