src/PlutusIR/Semantics/TypeSafety/TypeLanguage/StrongNormalisation.v
@@ -1,9 +1,9 @@
 Require Import PlutusCert.PlutusIR.Semantics.Static.
 Require Import PlutusCert.PlutusIR.Semantics.Static.Kinding.Checker.
 
-Require Import PlutusCert.PlutusIR.Semantics.Static.Normalisation.Normaliser_sound_complete.
+Require Import PlutusCert.PlutusIR.Semantics.Static.Normalization.Normalizer_sound_complete.
 
-From PlutusCert Require Import SN_PIR Normaliser.
+From PlutusCert Require Import SN_PIR Normalizer.
 
 Theorem strong_normalisation Δ T K :
     Δ |-* T : K ->
@@ -11,7 +11,7 @@ Theorem strong_normalisation Δ T K :
 Proof.
     intros Hkind.
     remember Hkind as Hkind'. clear HeqHkind'.
-    apply plutus_ty_strong_normalization in Hkind.
+    apply strong_normalization_PIR in Hkind.
     assert ({Tn & normalise T Tn}) as [Tn Hnorm].
     {
         eapply SN_normalise; eauto.
